src/Lean/Elab/Tactic/BVDecide/Frontend/Normalize/Rewrite.lean
@@ -53,7 +53,6 @@ where
     goal.withContext do
       -- TODO: it seems getNondepPropHyps doesn't return all the hyps we are interested in, investiagte
       let hyps ← goal.getNondepPropHyps
-      trace[Meta.Tactic.bv] m!"Filtering: {hyps.map mkFVar}"
       let filter hyp := do
         return !(← PreProcessM.checkRewritten hyp)
       hyps.filterM filter
